Speed up toposort
We are aiming for something like Kahn's algorithm, which is meant to
be O(|V| + |E|), but this requires mutability (which we can't do), or
at least functional maps (which we could do but would add a lot of
complexity).

The algorithm I have here is (I think) O(|V|^2), BUT tail
recursive (which the previous version wasn't) and with better constant
factors. Experimentation showed it's "Fast Enough"(TM), and it is
reasonable to prove correct, so we're sticking with it.

At this point, we are fast enough to not time out on the EPFL
benchmarks, so we're done with optimisation work for now.

Squashed commits
* Make VariableSet.of_list tail-recursive
* WIP Make module toposort tail-recursive
* Get VerilogEquivalenceCorrectness compiling
* WIP fast and correct module sorting
* Complete module sort specification

vera/Verilog.v
@@ -290,25 +290,66 @@ Variant bitwiseop :=
         congruence.
     Qed.
 
-    (* This is the version with nice recursion, which we want for inductive proofs, but is not tail-recursive *)
-    Equations of_list : list variable -> t := {
-      | [] => empty
-      | (x :: xs) => add x (of_list xs)
-    }.
+    Definition of_list (l : list variable) := fold_left (Basics.flip add) l empty.
 
-    (* This is the tail-recursive version, which we want for performance, but is annoying in proofs.
-       TODO: Profile and swap to this if we need it
-     *)
-    (* Definition of_list l := fold_right add empty l. *)
+    Lemma In_of_list_helper {a s l} :
+      (List.In a l \/ In a s) ->
+      In a (fold_left (Basics.flip add) l s).
+    Proof.
+      unfold Basics.flip.
+      revert a s.
+      induction l; intros *.
+      - intros [[]|H]. assumption.
+      - intros [[H|H]|H]; simpl.
+        + subst. apply IHl. right. fsetdec.
+	+ apply IHl. left. assumption.
+	+ apply IHl. fsetdec.
+    Qed.
+
+    Lemma In_of_list_helper2 {a s l} :
+      In a (fold_left (Basics.flip add) l s) ->
+      (List.In a l \/ In a s).
+    Proof.
+      unfold Basics.flip.
+      revert a s.
+      induction l; intros * H; [solve [auto]|].
+      simpl in H.
+      apply IHl in H. clear IHl. destruct H.
+      - left. right. exact H.
+      - destruct (dec (a0 = a)).
+        + subst. left. left. reflexivity.
+	+ right. fsetdec.
+    Qed.
 
     Lemma In_of_list {a l} :
-      List.In a l ->
-      In a (VariableSet.of_list l).
+      In a (of_list l) <-> List.In a l.
     Proof.
-      induction l; intros H; inv H.
-      all: simp of_list.
-      - fsetdec.
-      - insterU IHl. fsetdec.
+      unfold of_list.
+      split; intros.
+      - apply In_of_list_helper2 in H.
+        destruct H.
+	+ assumption.
+	+ fsetdec.
+      - apply In_of_list_helper.
+        left. assumption.
+    Qed.
+
+    Lemma of_list_cons {x l} :
+      Equal (of_list (x :: l)) (add x (of_list l)).
+    Proof.
+      unfold Equal.
+      split; intros H.
+      - rewrite In_of_list in H.
+        destruct H.
+	+ subst. fsetdec.
+	+ rewrite <- In_of_list in H.
+	  fsetdec.
+      - rewrite In_of_list.
+        destruct (dec (a = x)).
+        + subst. auto with datatypes.
+	+ right.
+	  rewrite <- In_of_list.
+	  fsetdec.
     Qed.
 
     Lemma subset_of_list {l1 l2} :
@@ -318,7 +359,7 @@ Variant bitwiseop :=
       revert l2. induction l1; intros l2 Hsub.
       - inv Hsub. fsetdec.
       - inv Hsub. fold (list_subset l1 l2) in *.
-        simp of_list.
+        rewrite of_list_cons.
 	insterU IHl1.
 	apply In_of_list in H1.
 	fsetdec.
